Revert "Simplify smallvec's model, removing later"
This reverts commit 8b842864dd7d2bdf128db060dd11431021e95b69.

theories/typing/lib/smallvec/smallvec.v
@@ -34,23 +34,24 @@ Section smallvec.
   Definition any_loc: loc := inhabitant.
 
   Lemma split_mt_smallvec {𝔄} (ty: type 𝔄) k l' tid d alπ Φ :
-    (l' ↦∗: (λ vl,
+    (l' ↦∗: (λ vl, [S(d') := d]
       ∃(b: bool) (l: loc) (len ex: nat) wl (aπl: vec (proph 𝔄) len),
       ⌜vl = [ #b; #l; #len; #ex] ++ wl ∧ length wl = k ∧ alπ = lapply aπl⌝ ∗
       if@ b then (* array mode *)
         ∃(wll: vec _ _) wl', ⌜wl = concat wll ++ wl'⌝ ∗
-          [∗ list] aπwl ∈ vzip aπl wll, ty.(ty_own) aπwl.1 d tid aπwl.2
-      else (* vector mode *) Φ l len ex aπl)) ⊣⊢
-    ∃(b: bool) (l: loc) (len ex: nat) (aπl: vec (proph 𝔄) len),
+          [∗ list] aπwl ∈ vzip aπl wll, ty.(ty_own) aπwl.1 d' tid aπwl.2
+      else (* vector mode *) Φ d' l len ex aπl)) ⊣⊢
+    [S(d') := d] ∃(b: bool) (l: loc) (len ex: nat) (aπl: vec (proph 𝔄) len),
       ⌜alπ = lapply aπl⌝ ∗ l' ↦∗ [ #b; #l; #len; #ex] ∗
       if@ b then (* array mode *)
-        ([∗ list] i ↦ aπ ∈ aπl, (l' +ₗ 4 +ₗ[ty] i) ↦∗: ty.(ty_own) aπ d tid) ∗
-        ∃wl', ⌜k = (len * ty.(ty_size) + length wl')%nat⌝ ∗ (l' +ₗ 4 +ₗ[ty] len) ↦∗ wl'
+        ([∗ list] i ↦ aπ ∈ aπl, (l' +ₗ 4 +ₗ[ty] i) ↦∗: ty.(ty_own) aπ d' tid) ∗
+          ∃wl', ⌜k = (len * ty.(ty_size) + length wl')%nat⌝ ∗ (l' +ₗ 4 +ₗ[ty] len) ↦∗ wl'
       else (* vector mode *)
-        ∃wl, ⌜length wl = k⌝ ∗ (l' +ₗ 4) ↦∗ wl ∗ Φ l len ex aπl.
+        ∃wl, ⌜length wl = k⌝ ∗ (l' +ₗ 4) ↦∗ wl ∗ Φ d' l len ex aπl.
   Proof.
     iSplit.
-    - iIntros "(%& ↦ & big)". iDestruct "big" as (b ?????(->&?&?)) "big".
+    - iIntros "(%& ↦ & big)". case d=>// ?.
+      iDestruct "big" as (b ?????(->&?&?)) "big".
       iExists _, _, _, _, _. iSplit; [done|].
       rewrite !heap_mapsto_vec_cons heap_mapsto_vec_nil !shift_loc_assoc.
       iDestruct "↦" as "($&$&$&$& ↦)". case b; [|iExists _; by iFrame].
@@ -59,7 +60,8 @@ Section smallvec.
       rewrite heap_mapsto_vec_app trans_big_sepL_mt_ty_own shift_loc_assoc.
       iDestruct "↦" as "[? ↦ex]". iSplitR "↦ex"; iExists _; iFrame.
       by rewrite -app_length.
-    - iDestruct 1 as (b ?????) "(↦hd & big)". case b.
+    - iIntros "big". case d=>// ?.
+      iDestruct "big" as (b ?????) "(↦hd & big)". case b.
       + rewrite trans_big_sepL_mt_ty_own.
         iDestruct "big" as "[(%wll & ↦ar & tys) (%wl' &->& ↦ex)]".
         iDestruct (big_sepL_ty_own_length with "tys") as %Eqsz.
@@ -78,42 +80,48 @@ Section smallvec.
   Program Definition smallvec {𝔄} (n: nat) (ty: type 𝔄) : type (listₛ 𝔄) := {|
     ty_size := 4 + n * ty.(ty_size);
     ty_lfts := ty.(ty_lfts);  ty_E := ty.(ty_E);
-    ty_own alπ d tid vl :=
+    ty_own alπ d tid vl := [S(d') := d]
       ∃(b: bool) (l: loc) (len ex: nat) wl (aπl: vec (proph 𝔄) len),
         ⌜vl = [ #b; #l; #len; #ex] ++ wl
           ∧ length wl = (n * ty.(ty_size))%nat ∧ alπ = lapply aπl⌝ ∗
         if@ b then (* array mode *)
           ∃(wll: vec _ _) wl', ⌜wl = concat wll ++ wl'⌝ ∗
-            [∗ list] aπwl ∈ vzip aπl wll, ty.(ty_own) aπwl.1 d tid aπwl.2
+            [∗ list] aπwl ∈ vzip aπl wll, ty.(ty_own) aπwl.1 d' tid aπwl.2
         else (* vector mode *)
-          ([∗ list] i ↦ aπ ∈ aπl, (l +ₗ[ty] i) ↦∗: ty.(ty_own) aπ d tid) ∗
+          ▷ ([∗ list] i ↦ aπ ∈ aπl, (l +ₗ[ty] i) ↦∗: ty.(ty_own) aπ d' tid) ∗
           (l +ₗ[ty] len) ↦∗len (ex * ty.(ty_size)) ∗
           freeable_sz' ((len + ex) * ty.(ty_size)) l;
     ty_shr alπ d κ tid l' :=
-      ∃(b: bool) (l: loc) (len ex: nat) (aπl: vec (proph 𝔄) len),
+      [S(d') := d] ∃(b: bool) (l: loc) (len ex: nat) (aπl: vec (proph 𝔄) len),
         ⌜alπ = lapply aπl⌝ ∗
         &frac{κ} (λ q, l' ↦∗{q} [ #b; #l; #len; #ex]) ∗
         if@ b then (* array mode *)
-          [∗ list] i ↦ aπ ∈ aπl, ty.(ty_shr) aπ d κ tid (l' +ₗ 4 +ₗ[ty] i)
+          [∗ list] i ↦ aπ ∈ aπl, ty.(ty_shr) aπ d' κ tid (l' +ₗ 4 +ₗ[ty] i)
         else (* vector mode *)
-          [∗ list] i ↦ aπ ∈ aπl, ty.(ty_shr) aπ d κ tid (l +ₗ[ty] i);
+          ▷ [∗ list] i ↦ aπ ∈ aπl, ty.(ty_shr) aπ d' κ tid (l +ₗ[ty] i);
   |}%I.
-  Next Obligation. iDestruct 1 as (??????(->&Eq&_)) "svec/=". by rewrite Eq. Qed.
   Next Obligation.
-    move=> */=. do 21 f_equiv; [f_equiv|]; apply ty_own_depth_mono; lia.
+    iIntros (????[]??) "svec //". iDestruct "svec" as (??????(->&Eq&_)) "?/=".
+    by rewrite Eq.
   Qed.
   Next Obligation.
-    move=> */=. do 16 f_equiv; apply ty_shr_depth_mono; lia.
+    move=> ???[|?][|?]*/=; try (by iIntros); [lia|].
+    do 22 f_equiv; apply ty_own_depth_mono; lia.
   Qed.
   Next Obligation.
-    iIntros "%%* #? (%b &%&%&%&%&%&?& All)". iExists b, _, _, _, _.
-    iSplit; [done|]. iSplit; [by iApply frac_bor_shorten|].
-    case b=>/=; rewrite !big_sepL_forall;
+    move=> ???[|?][|?]*/=; try (by iIntros); [lia|].
+    do 16 f_equiv; [|f_equiv]; apply ty_shr_depth_mono; lia.
+  Qed.
+  Next Obligation.
+    move=> ??????[|?]*; [by iIntros|]. iIntros "#? (%b &%&%&%&%&%&?& All)".
+    iExists b, _, _, _, _. iSplit; [done|]. iSplit; [by iApply frac_bor_shorten|].
+    case b=>/=; rewrite !big_sepL_forall; [|iNext];
     iIntros "**"; iApply ty_shr_lft_mono; by [|iApply "All"].
   Qed.
   Next Obligation.
-    iIntros "*% #LFT In Bor κ". rewrite split_mt_smallvec.
-    iMod (bor_exists with "LFT Bor") as (b) "Bor"; [done|].
+    iIntros (? n ty ?? d ? l tid ??) "#LFT In Bor κ". rewrite split_mt_smallvec.
+    case d. { by iMod (bor_persistent with "LFT Bor κ") as "[>[] _]". }
+    move=> ?. iMod (bor_exists with "LFT Bor") as (b) "Bor"; [done|].
     do 4 (iMod (bor_exists_tok with "LFT Bor κ") as (?) "[Bor κ]"; [done|]).
     iMod (bor_sep_persistent with "LFT Bor κ") as "(>-> & Bor & κ)"; [done|].
     iMod (bor_sep with "LFT Bor") as "[Bor↦ Bor]"; [done|].
@@ -121,26 +129,29 @@ Section smallvec.
     case b=>/=.
     - iMod (bor_sep with "LFT Bor") as "[Bor _]"; [done|].
       iMod (ty_share_big_sepL with "LFT In Bor κ") as "Toshrs"; [done|].
-      iApply (step_fupdN_wand with "Toshrs"). iIntros "!> >[?$] !>".
+      iApply (step_fupdN_wand with "Toshrs"). iIntros "!>!>!>!> >[?$] !>".
       iExists true, _, _, _, _. by iFrame.
     - iMod (bor_exists with "LFT Bor") as (?) "Bor"; [done|].
       iMod (bor_sep_persistent with "LFT Bor κ") as "(_ & Bor & κ)"; [done|].
       iMod (bor_sep with "LFT Bor") as "[_ Bor]"; [done|].
       iMod (bor_sep with "LFT Bor") as "[Bor _]"; [done|].
+      iMod (bor_later_tok with "LFT Bor κ") as "Borκ"; [done|].
+      iIntros "/=!>!>!>". iMod "Borκ" as "[Bor κ]".
       iMod (ty_share_big_sepL with "LFT In Bor κ") as "Toshrs"; [done|].
       iApply (step_fupdN_wand with "Toshrs"). iIntros "!> >[?$] !>".
       iExists false, _, _, _, _. iFrame "Bor↦". by iSplit.
   Qed.
   Next Obligation.
-    iIntros "*% LFT In svec κ". iDestruct "svec" as (b ?????(->&?&->)) "big". case b=>/=.
+    iIntros (?????[|?]) "*% LFT In svec κ/="; [done|].
+    iDestruct "svec" as (b ?????(->&?&->)) "big". case b=>/=.
     - iDestruct "big" as (??->) "tys".
       iMod (ty_own_proph_big_sepL with "LFT In tys κ") as "Upd"; [done|].
-      iApply (step_fupdN_wand with "Upd"). iIntros "!> >(%&%&%& ξl & Totys) !>".
-      iExists _, _. iSplit.
+      iApply (step_fupdN_wand with "Upd").
+      iIntros "!>!>!>!> >(%&%&%& ξl & Totys) !>". iExists _, _. iSplit.
       { iPureIntro. rewrite -vec_to_list_apply. by apply proph_dep_constr. }
       iIntros "{$ξl}ξl". iMod ("Totys" with "ξl") as "[? $]". iModIntro.
       iExists true, _, _, _, _, _. iSplit; [done|]. iExists _, _. by iFrame.
-    - iDestruct "big" as "(↦tys & ex & †)".
+    - iDestruct "big" as "(↦tys & ex & †)". iIntros "!>!>!>".
       iMod (ty_own_proph_big_sepL_mt with "LFT In ↦tys κ") as "Upd"; [done|].
       iApply (step_fupdN_wand with "Upd"). iIntros "!> >(%&%&%& ξl & Totys) !>".
       iExists _, _. iSplit.
@@ -149,8 +160,8 @@ Section smallvec.
       iExists false, _, _, _, _, _. iSplit; [done|]. iFrame.
   Qed.
   Next Obligation.
-    iIntros "%%*% LFT In In' svec κ'". iDestruct "svec" as (b ????->) "[? tys]".
-    case b=>/=.
+    iIntros (?????[|?]) "*% LFT In In' svec κ'/="; [done|].
+    iDestruct "svec" as (b ????->) "[? tys]". case b=>/=; iIntros "!>!>!>".
     - iMod (ty_shr_proph_big_sepL with "LFT In In' tys κ'") as "Upd"; [done|].
       iIntros "!>!>". iApply (step_fupdN_wand with "Upd").
       iIntros ">(%&%&%& ξl & Totys) !>". iExists _, _. iSplit.
